Cslib/Languages/Boole/examples/Boogie/arithm/expansion.lean
@@ -1,5 +1,4 @@
 import Strata.MetaVerifier
-import Smt
 
 namespace Strata
 
