Cslib/Languages/Boole/examples/Boogie/arithm/fundef.lean
@@ -30,6 +30,6 @@ spec {
 
 example : Strata.smtVCsCorrect funDef := by
   gen_smt_vcs
-  all_goals (smt +mono)
+  all_goals smt +mono
 
 end Strata
