Cslib/Languages/Boole/examples/Boogie/codeexpr/codeexpr.lean
@@ -1,4 +1,5 @@
 import Strata.MetaVerifier
+import Smt
 
 namespace Strata
 
@@ -65,6 +66,6 @@ procedure D(a : (Map int T), n : int) returns ()
 
 example : Strata.smtVCsCorrect codeExpr := by
   gen_smt_vcs
-  all_goals grind
+  all_goals smt +mono
 
 end Strata
