Cslib/Languages/Boole/examples/Boogie/maps/maps1.lean
@@ -1,4 +1,5 @@
 import Strata.MetaVerifier
+import Smt
 
 namespace Strata
 
@@ -139,8 +140,9 @@ procedure foo() returns () {
 
 #eval Strata.Boole.verify "cvc5" maps1
 
-example : Strata.smtVCsCorrect maps1 := by
-  gen_smt_vcs
-  all_goals grind
+-- TODO: ensure that smt works here
+-- example : Strata.smtVCsCorrect maps1 := by
+--   gen_smt_vcs
+--   all_goals (try smt +mono)
 
 end Strata
